theories/TM/Code/List/Rev.v
@@ -1,4 +1,4 @@
-From Undecidability Require Import ProgrammingTools.
+From Undecidability.TM Require Import ProgrammingTools.
 From Undecidability Require Import CaseNat CaseList CaseSum Hoare. (* [TM.Code.CaseSum] contains [Constr_Some] and [Constr_None]. *)
 
 
