theories/TM/Combinators/If.v
@@ -1,4 +1,4 @@
-From Undecidability Require Import Switch.
+From Undecidability.TM Require Import Util.TM_facts Switch.
 
 Section If.
 
