theories/TM/Hoare/HoareCombinators.v
@@ -1,7 +1,7 @@
 (* ** Some Hoare Rules *)
 
 From Undecidability Require Import TMTac TM.Util.Prelim.
-From Undecidability Require Export TM.Compound.Multi TM.Combinators.Combinators.
+From Undecidability.TM Require Export Compound.Multi Combinators.Combinators.
 From Undecidability.TM.Hoare Require Import HoareLogic HoareRegister.
 
 (* *** Nop *)
